raft/proof/LastAppliedCommitIndexMatchingProof.v
@@ -111,10 +111,55 @@ Section LastAppliedCommitIndexMatching.
         simpl in *; intuition.
   Qed.
   
+  Theorem lastApplied_lastApplied_match_invariant :
+    forall net,
+      raft_intermediate_reachable net ->
+      lastApplied_lastApplied_match net.
+  Proof.
+    intros.
+    find_copy_apply_lem_hyp log_matching_invariant. unfold log_matching in *.
+    find_copy_apply_lem_hyp state_machine_safety_invariant. unfold state_machine_safety in *.
+    find_copy_apply_lem_hyp max_index_sanity_invariant. unfold maxIndex_sanity in *.
+    unfold lastApplied_lastApplied_match.
+    intuition; simpl in *.
+    - unfold log_matching_hosts in *. intuition. simpl in *.
+      match goal with
+        | H : forall (_ : name) (_ : nat), _ |- In ?e (_ (_ ?h)) =>
+          specialize (H h (eIndex e)); forward H;
+          intuition
+      end.
+      + find_apply_hyp_hyp; omega.
+      + eapply le_trans; [|eapply_prop maxIndex_lastApplied].
+        simpl. omega.
+      + break_exists. intuition.
+        match goal with
+          | _ : eIndex ?e = eIndex ?e' |- _ =>
+            cut (e = e'); [intros; subst; auto|]
+        end.
+        eapply_prop state_machine_safety_host; unfold commit_recorded; intuition eauto;
+        simpl in *; intuition.
+    - unfold log_matching_hosts in *. intuition. simpl in *.
+      match goal with
+        | H : forall (_ : name) (_ : nat), _ |- In ?e (_ (_ ?h)) =>
+          specialize (H h (eIndex e)); forward H;
+          intuition
+      end.
+      + find_apply_hyp_hyp; omega.
+      + eapply le_trans; [|eapply_prop maxIndex_lastApplied].
+        simpl. omega.
+      + break_exists. intuition.
+        match goal with
+          | _ : eIndex ?e = eIndex ?e' |- _ =>
+            cut (e = e'); [intros; subst; auto|]
+        end.
+        eapply_prop state_machine_safety_host; unfold commit_recorded; intuition eauto;
+        simpl in *; intuition.
+  Qed.
 
   Instance lacimi : lastApplied_commitIndex_match_interface.
   split.
   - exact lastApplied_commitIndex_match_invariant.
   - exact commitIndex_lastApplied_match_invariant.
+  - exact lastApplied_lastApplied_match_invariant.
   Defined.
 End LastAppliedCommitIndexMatching.
